program_logic/sts.v
@@ -100,7 +100,6 @@ Section sts.
     rewrite /sts_inv later_exist sep_exist_r. apply exist_elim=>s.
     rewrite later_sep pvs_timeless !pvs_frame_r. apply pvs_mono.
     rewrite -(exist_intro s). ecancel [▷ φ _]%I.
-    to_front [own _ _; sts_ownS _ _ _].
     rewrite -own_op own_valid_l discrete_valid.
     apply const_elim_sep_l=> Hvalid.
     assert (s ∈ S) by eauto using sts_auth_frag_valid_inv.
